add: changed hard-coded maxPriority in the priority queue

source/PriorityQueue.dfy
@@ -1,96 +1,74 @@
 include "Signal.dfy"
 include "Queue.dfy"
 
-const maxPriority := 3;
-
-function emptyLists<T>() : seq<seq<T>>
-	ensures |emptyLists<T>()| == maxPriority
-	ensures forall i :: 0 <= i < maxPriority ==> emptyLists<T>()[i] == []
-	ensures flatten(emptyLists<T>()) == []
+function emptyLists<T>(size : nat) : seq<seq<T>>
+	ensures |emptyLists<T>(size)| == size
+	ensures forall i :: 0 <= i < size ==> emptyLists<T>(size)[i] == []
+	ensures flatten<T>(emptyLists<T>(size)) == []
 {
-	[[], [], []]
+	if size == 0 then
+		[]
+	else
+		[[]] + emptyLists(size - 1)
 }
 
 function flatten<T>(sequences : seq<seq<T>>) : seq<T>
-	requires |sequences| == maxPriority
 {
-	sequences[0] + sequences[1] + sequences[2]
+	if |sequences| == 0 then
+		[]
+	else
+		sequences[0] + flatten(sequences[1..])
 }
 
 function firstNonEmpty<T>(sequences : seq<seq<T>>) : nat
-	requires |sequences| == maxPriority
-	requires flatten(sequences) != []
-	ensures 0 <= firstNonEmpty(sequences) < |sequences|
-	ensures |sequences[firstNonEmpty(sequences)]| > 0
+	requires flatten<T>(sequences) != []
+	ensures 0 <= firstNonEmpty<T>(sequences) < |sequences|
+	ensures |sequences[firstNonEmpty<T>(sequences)]| > 0
 	ensures forall k :: 0 <= k < |sequences| && sequences[k] != []
-	==> firstNonEmpty(sequences) <= k
+	==> firstNonEmpty<T>(sequences) <= k
 {
-	assert sequences[0] != [] || sequences[1] != [] || sequences[2] != [];
 	if sequences[0] != [] then
 		0
-	else if sequences[1] != [] then
-		1
 	else
-		2
+		1 + firstNonEmpty(sequences[1..])
 }
 
 function addTo<T>(sequences : seq<seq<T>>, priority : nat, value : T) : seq<seq<T>>
-	requires 0 < priority <= maxPriority
-	requires |sequences| == maxPriority
-	ensures |addTo(sequences, priority, value)| == maxPriority
-	ensures forall i :: 0 <= i < maxPriority && i != index(priority) ==> addTo(sequences, priority, value)[i] == sequences[i]
+	requires 0 < priority <= |sequences|
+	ensures |addTo(sequences, priority, value)| == |sequences|
+	ensures forall i :: 0 <= i < |sequences| && i != index(priority) ==> addTo(sequences, priority, value)[i] == sequences[i]
 	ensures addTo(sequences, priority, value)[index(priority)] == sequences[index(priority)] + [value] 
 {
 	var changeIndex := index(priority);
-	var seq0 := if changeIndex == 0 then
-		sequences[0] + [value]
+	if changeIndex == 0 then
+		[sequences[0] + [value]] + sequences[1..]
 	else
-		sequences[0];
-		var seq1 := if changeIndex == 1 then
-			sequences[1] + [value]
-		else
-			sequences[1];
-			var seq2 := if changeIndex == 2 then
-				sequences[2] + [value]
-	else
-		sequences[2];
-		[seq0, seq1, seq2]
+		[sequences[0]] + addTo(sequences[1..], priority - 1, value)
 }
 
 function removeFrom<T>(sequences : seq<seq<T>>, priority : nat) : seq<seq<T>>
-	requires 0 < priority <= maxPriority
-	requires |sequences| == maxPriority
+	requires 0 < priority <= |sequences|
 	requires |sequences[index(priority)]| > 0 
-	ensures |removeFrom(sequences, priority)| == maxPriority
-	ensures forall i :: 0 <= i < maxPriority && i != index(priority) ==> removeFrom(sequences, priority)[i] == sequences[i]
+	ensures |removeFrom(sequences, priority)| == |sequences|
+	ensures forall i :: 0 <= i < |sequences| && i != index(priority) ==> removeFrom(sequences, priority)[i] == sequences[i]
 	ensures removeFrom(sequences, priority)[index(priority)] == sequences[index(priority)][1..]
 {
 	var changeIndex := index(priority);
-	var seq0 := if changeIndex == 0 then
-		sequences[0][1..]
+	if changeIndex == 0 then
+		[sequences[0][1..]] + sequences[1..]
 	else
-		sequences[0];
-		var seq1 := if changeIndex == 1 then
-			sequences[1][1..]
-	else
-		sequences[1];
-		var seq2 := if changeIndex == 2 then
-			sequences[2][1..]
-	else
-		sequences[2];
-		[seq0, seq1, seq2]
+		[sequences[0]] + removeFrom(sequences[1..], priority - 1)
 }
 
 function method index(priority : nat) : nat
-	requires 0 < priority <= maxPriority
-	ensures 0 <= index(priority) < maxPriority
+	requires 0 < priority
+	ensures 0 <= index(priority)
 {
 	priority - 1
 }
 
 function priority(index : nat) : nat
-	requires 0 <= index < maxPriority
-	ensures 0 < priority(index) <= maxPriority
+	ensures 0 < priority(index)
 {
 	index + 1
 }
@@ -98,42 +76,53 @@ function priority(index : nat) : nat
 
 class {:autocontracts} PriorityQueue
 {
-	var queue0 : Queue;
-	var queue1 : Queue;
-	var queue2 : Queue;
+	const maxPriority : nat;
+	var queues : array<Queue>;
 	var elements : nat;
 	ghost var sequences : seq<seq<Signal>>;
 
-	constructor(default : Signal)
-		ensures sequences == emptyLists()
+	constructor(maxPriority : nat, default : Signal)
+		requires maxPriority > 0
+		ensures sequences == emptyLists(maxPriority)
 		ensures flatten(sequences) == []
+		ensures this.maxPriority == maxPriority
 	{
+		this.maxPriority := maxPriority;
+		new;
+		var dummyQueue := new Queue(default);
+		var queuesI : array<Queue> := new Queue[maxPriority](_ => dummyQueue);
+		var i := 0;
+		while i < maxPriority
+			invariant 0 <= i <= maxPriority
+			invariant forall j :: 0 <= j < i ==> queuesI[j].Valid()
+			invariant forall j :: 0 <= j < i ==> queuesI[j].elemSeq == []
+			invariant forall j, k :: 0 <= j < k < i ==> queuesI[j] != queuesI[k]
+			invariant forall j, k :: 0 <= j < k < i ==> queuesI[j].elements != queuesI[k].elements
+		{
+			queuesI[i] := new Queue(default);
+			i := i + 1;
+		}
+		queues := queuesI;
 		this.elements := 0;
-		this.queue0 := new Queue(default);
-		this.queue1 := new Queue(default);
-		this.queue2 := new Queue(default);
-		this.sequences := emptyLists();
-	} 
+		this.sequences := emptyLists(maxPriority);
+		assert |sequences| == maxPriority;
+		assert elements == |flatten(sequences)|;
+		assert forall i :: 0 <= i < maxPriority ==> queues[i].Valid();
+		assert forall i, j :: 0 <= i < j < maxPriority ==> queues[i] != queues[j];
+		assert forall i :: 0 <= i < maxPriority ==> sequences[i] == queues[i].elemSeq;
+		assert forall i, j :: 0 <= i < j < maxPriority ==> queues[i].elements != queues[j].elements;
+	}
 
 	predicate Valid()
 	{
 		&& |sequences| == maxPriority
+		&& queues.Length == maxPriority
 		&& elements == |flatten(sequences)|
-		&& queue0.Valid()
-		&& queue1.Valid()
-		&& queue2.Valid()
-		&& queue0 != queue1
-		&& queue1 != queue2
-		&& queue2 != queue0
-		&& queue0.elements != queue1.elements
-		&& queue1.elements != queue2.elements
-		&& queue2.elements != queue0.elements
-		&& queue0.Repr * queue1.Repr == {}
-		&& queue1.Repr * queue2.Repr == {}
-		&& queue2.Repr * queue0.Repr == {}
-		&& sequences[0] == queue0.elemSeq
-		&& sequences[1] == queue1.elemSeq
-		&& sequences[2] == queue2.elemSeq	
+		&& (forall i :: 0 <= i < maxPriority ==> queues[i].Valid())
+		&& (forall i, j :: 0 <= i < j < maxPriority ==> queues[i] != queues[j])
+		&& (forall i, j :: 0 <= i < j < maxPriority ==> queues[i].elements != queues[j].elements)
+		&& (forall i, j :: 0 <= i < j < maxPriority ==> queues[i].Repr * queues[j].Repr == {})
+		&& (forall i :: 0 <= i < maxPriority ==> sequences[i] == queues[i].elemSeq)
 	}
 	
 	function method size() : nat
@@ -157,21 +146,27 @@ class {:autocontracts} PriorityQueue
 	{
 		priority(firstNonEmpty(sequences))
 	}
-
-	function method minPriority() : nat
+	
+	method minPriority() returns (min : nat)
 		requires !empty()
-		ensures minPriority() == minPriorityFunc()
-		ensures 0 < minPriority() <= maxPriority
-		ensures |sequences[index(minPriority())]| > 0
+		ensures min == minPriorityFunc()
+		ensures 0 < min <= maxPriority
+		ensures |sequences[index(min)]| > 0
 		ensures forall k :: 0 <= k < |sequences| && sequences[k] != []
-		==> index(minPriority()) <= k
+		==> index(min) <= k
 	{
-		if queue0.size() > 0 then
-			1
-		else if queue1.size() > 0 then
-			2
-		else
-			3
+		var i := 0;
+		while i < maxPriority
+			invariant 0 <= i <= maxPriority
+			invariant forall j :: 0 <= j < i ==> queues[j].size() == 0
+		{
+			if queues[i].size() > 0
+			{
+				min := i + 1;
+				break;
+			}
+			i := i + 1;
+		}
 	}
 	
 	method push(value : Signal, priority : nat)
@@ -182,14 +177,7 @@ class {:autocontracts} PriorityQueue
 		==> sequences[k] == old(sequences[k])
 	{
 		var queueIndex := index(priority);
-		if queueIndex == 0 {
-			queue0.push(value);
-		} else if queueIndex == 1 {
-			queue1.push(value);
-		} else if queueIndex == 2 {
-			queue2.push(value);
-		}
-
+		queues[queueIndex].push(value);
 		elements := elements + 1;
 		sequences := addTo(sequences, priority, value);
 	}
@@ -204,38 +192,25 @@ class {:autocontracts} PriorityQueue
 	{
 		var priority := minPriority();
 		var queueIndex := index(priority);
-		
-		if queueIndex == 0 {
-			result := queue0.pop();
-		} else if queueIndex == 1 {
-			result := queue1.pop();
-		} else if queueIndex == 2 {
-			result := queue2.pop();
-		}
-
+		result := queues[queueIndex].pop();
 		elements := elements - 1;
 		sequences := removeFrom(sequences, priority);
 	}
 
-	function method peek() : Signal
+	method peek() returns (result : Signal)
 		requires !empty()
-		ensures peek() == sequences[index(minPriorityFunc())][0]
+		ensures result == sequences[index(minPriorityFunc())][0]
 	{
 		var priority := minPriority();
 		var queueIndex := index(priority);
-		
-		if queueIndex == 0 then
-			queue0.peek()
-		else if queueIndex == 1 then
-			queue1.peek()
-		else
-			queue2.peek()
+		result := queues[queueIndex].peek();
 	}
 }
 
+/*
 method TestPriorityQueue()
 {
-	var q := new PriorityQueue(Reverse(false));
+	var q := new PriorityQueue(3, Reverse(false));
 	q.push(Brake(2), 1);
 	q.push(Beam(20), 3);
 	q.push(Brake(5), 2);
@@ -247,4 +222,4 @@ method TestPriorityQueue()
 	assert y == Brake(5);
 	y := q.pop();
 	assert y == Beam(20);
-}
+}*/
